Labeled using lists with permutations

LLSemantics.v
@@ -1,23 +1,11 @@
 Require Import LLSubstitution.
 Require Import PermutLib.
+Require Import LibTactics.
+Require Import LLOkLib.
 
 Open Scope is5_scope.
 Open Scope labeled_is5_scope.
 Open Scope permut_scope.
-
-Fixpoint ok_Gamma (G: Context_L) (Used: list var) : Prop :=
-match G with
-| nil => True
-| (w, (v, A)) :: G' => ~ Mem v Used /\ ok_Gamma G' (v::Used)
-end.
-
-Fixpoint ok_Omega (L: list var) : Prop :=
-match L with
-| nil => True
-| l :: L' => ~ Mem l L' /\ ok_Omega L'
-end.
-
-Definition ok_L Omega Gamma := ok_Omega Omega /\ok_Gamma Gamma nil.
 
 Global Reserved Notation " Omega ';' Gamma '|-' M ':::' A '@' w " (at level 70).
 
@@ -53,17 +41,19 @@ Inductive types_L: worlds_L -> Context_L -> te_L -> ty -> var -> Prop :=
 
 | t_fetch_L: forall Omega Gamma w w' M A
   (Ok: ok_L Omega Gamma)
-  (HT: Omega; Gamma |- M ::: [*]A @ w),
+  (HT: Omega; Gamma |- M ::: [*]A @ w)
+  (Hin: Mem w' Omega),
   Omega; Gamma |- fetch_L (fwo w) M ::: [*]A @ w'
 
 | t_here: forall Omega Gamma w M A
   (Ok: ok_L Omega Gamma)
-  (HT: Omega; Gamma |- M ::: <*>A @ w),
-  Omega; Gamma |- here_L M ::: A @ w
+  (HT: Omega; Gamma |- M ::: A @ w),
+  Omega; Gamma |- here_L M ::: <*> A @ w
 
 | t_get_L: forall Omega Gamma w w' M A
   (Ok: ok_L Omega Gamma)
-  (HT: Omega; Gamma |- M ::: <*>A @ w),
+  (HT: Omega; Gamma |- M ::: <*>A @ w)
+  (Hin: Mem w' Omega),
   Omega; Gamma |- get_L (fwo w) M ::: <*>A @ w'
 
 | t_letd_L: forall Lw Lt Omega Gamma w M N A B
@@ -85,18 +75,17 @@ Inductive value_L: te_L -> Prop :=
 
 Global Reserved Notation " M |-> N " (at level 70).
 
-
-Inductive step_LF: te_L * vwo -> te_L * vwo -> Prop :=
+Inductive step_L: te_L * vwo -> te_L * vwo -> Prop :=
 | red_appl_lam_L: forall A M N w,
-   lc_t_L M -> lc_w_L (M ^t^ N) ->
-   lc_t_L N -> lc_w_L N ->
+   lc_w_L M -> lc_t_L (M ^t^ N) ->
+   lc_w_L N -> lc_t_L N ->
    (appl_L (lam_L A M) N, w) |-> (M ^t^ N, w)
 | red_unbox_box_L: forall M w,
    lc_t_L M -> lc_w_L (M ^w^ w) ->
    (unbox_L (box_L M), w) |-> (M ^w^ w, w)
 | red_letd_here_L: forall M N w (HVal: value_L M),
    lc_t_L M -> lc_w_L M ->
-   lc_t_L N ^t^ M -> lc_w_L (N ^w^ w) ->
+   lc_t_L (N ^t^ M) -> lc_w_L (N ^w^ w) ->
    (letd_L (here_L M) N, w) |-> ((N ^w^ w) ^t^ M, w)
 | red_appl_L: forall M N M' w (HRed: (M, w) |-> (M', w)),
    lc_t_L M -> lc_w_L M ->
@@ -124,8 +113,174 @@ Inductive step_LF: te_L * vwo -> te_L * vwo -> Prop :=
 | red_get_val_L: forall w M w' (HVal: value_L M),
    lc_t_L M -> lc_w_L M ->
    (get_L w (here_L M), w') |-> (here_L {{w'//w}}M, w')
-where " M |-> N " := (step_LF M N ) : labeled_is5_scope.
+where " M |-> N " := (step_L M N ) : labeled_is5_scope.
 
+Lemma WeakeningGamma:
+forall Omega Gamma M A w Gamma'
+  (H: Omega; Gamma |- M ::: A @ w)
+  (Ok: ok_L Omega (Gamma ++ Gamma')),
+  forall Delta,
+    Delta *=* Gamma ++ Gamma' ->
+    Omega; Delta |- M ::: A @ w.
+intros; generalize dependent Gamma'; generalize dependent Delta;
+induction H; intros.
+(* hyp *)
+constructor;
+[ eapply ok_L_permut; [ | symmetry | ] |
+  eapply Mem_permut; [ symmetry | rewrite Mem_app_or_eq; left ]]; eauto.
+(* lam *)
+apply t_lam_L with (L:=L \u used_vars_context_L (Gamma++Gamma')).
+  eapply ok_L_permut; [ | symmetry | ]; eauto.
+  intros; apply H with (Gamma':=Gamma'); auto; rew_app;
+  [ apply ok_L_extend_fresh | permut_simpl]; auto.
+(* appl *)
+apply t_appl_L with (A:=A).
+  eapply ok_L_permut; [ | symmetry | ]; eauto.
+  apply IHtypes_L1 with (Gamma':=Gamma'); auto.
+  apply IHtypes_L2 with (Gamma':=Gamma'); auto.
+(* box *)
+apply t_box_L with (L:=L \u from_list Omega).
+  eapply ok_L_permut; [ | symmetry | ]; eauto.
+  intros; apply H with (Gamma':=Gamma'); auto.
+  destruct Ok0; split; auto; simpl; split; [apply notin_Mem | ]; auto.
+(* unbox *)
+constructor; auto.
+  eapply ok_L_permut; [ | symmetry | ]; eauto.
+  apply IHtypes_L with (Gamma' := Gamma'); auto.
+(* fetch *)
+constructor; auto.
+  eapply ok_L_permut; [ | symmetry | ]; eauto.
+  apply IHtypes_L with (Gamma' := Gamma'); auto.
+(* here *)
+constructor; auto.
+  eapply ok_L_permut; [ | symmetry | ]; eauto.
+  apply IHtypes_L with (Gamma' := Gamma'); auto.
+(* get *)
+constructor; auto.
+  eapply ok_L_permut; [ | symmetry | ]; eauto.
+  apply IHtypes_L with (Gamma' := Gamma'); auto.
+(* letdia *)
+apply t_letd_L with (Lt := Lt \u used_vars_context_L (Gamma++Gamma'))
+  (Lw := Lw \u from_list Omega) (A := A); auto.
+  eapply ok_L_permut; [ | symmetry | ]; eauto.
+  apply IHtypes_L with (Gamma' := Gamma'); auto.
+  intros; apply H0 with (Gamma' := Gamma'); auto.
+  rew_app; apply ok_L_extend_fresh; destruct Ok0.
+    split; auto. simpl; split; [apply notin_Mem | ]; auto.
+    auto.
+  rew_app; permut_simpl; assumption.
+Qed.
+
+Lemma WeakeningOmega:
+forall Omega Gamma M A w w'
+  (H: Omega; Gamma |- M ::: A @ w)
+  (Ok: ok_L (w'::Omega) Gamma),
+  forall Omega',
+    Omega' *=* w'::Omega ->
+    Omega'; Gamma |- M ::: A @ w.
+intros Omega Gamma M A w w' H; generalize dependent w'; induction H; intros.
+(* hyp *)
+constructor; auto;
+eapply ok_L_permut with (O:=w'::Omega); [symmetry | | ]; eauto.
+(* lam *)
+apply t_lam_L with (L:=L \u used_vars_context_L Gamma).
+eapply ok_L_permut with (O:=w'::Omega); [symmetry | | ]; eauto.
+intros; eapply H; eauto.
+apply ok_L_extend_fresh; destruct Ok0; auto; split; auto.
+(* appl *)
+apply t_appl_L with (A:=A); eauto.
+eapply ok_L_permut with (O:=w'::Omega); [symmetry | | ]; eauto.
+(* box *)
+apply t_box_L with (L:=L \u from_list (w'::Omega)).
+  eapply ok_L_permut with (O:=w'::Omega); [symmetry | | ]; eauto.
+  intros; apply H with (w':=w'); auto.
+  eapply ok_L_permut with (O:=(x::w'::Omega)); eauto.
+    permut_simpl.
+    destruct Ok0; split; auto; simpl. split; auto.
+    apply notin_Mem; eauto.
+    permut_simpl; auto.
+(* unbox *)
+constructor; eauto.
+eapply ok_L_permut with (O:=w'::Omega); [symmetry | | ]; eauto.
+(* fetch *)
+constructor; eauto.
+eapply ok_L_permut with (O:=w'0::Omega); [symmetry | | ]; eauto.
+apply Mem_permut with (l:=w'0::Omega); rew_app;
+[ symmetry | rewrite Mem_cons_eq; right]; auto.
+(* here *)
+constructor; eauto.
+eapply ok_L_permut with (O:=w'::Omega); [symmetry | | ]; eauto.
+(* get *)
+constructor; eauto.
+eapply ok_L_permut with (O:=w'0::Omega); [symmetry | | ]; eauto.
+apply Mem_permut with (l:=w'0::Omega); rew_app;
+[ symmetry | rewrite Mem_cons_eq; right]; auto.
+(* letd *)
+apply t_letd_L with (Lt := Lt \u used_vars_context_L Gamma)
+  (Lw := Lw \u from_list (w'::Omega)) (A := A).
+  eapply ok_L_permut with (O:=w'::Omega); [symmetry | | ]; eauto.
+  apply IHtypes_L with (w' := w'); auto.
+  intros; apply H0 with (w' := w'0) (w'0 := w'); auto.
+  eapply ok_L_permut with (O:=w'0::w'::Omega).
+  permut_simpl. eauto.
+  apply ok_L_extend_fresh; destruct Ok0.
+    split; auto. simpl; split; [apply notin_Mem | ]; auto.
+    auto.
+  permut_simpl; assumption.
+Qed.
+
+Lemma PermutOmega:
+forall Omega Gamma M A w Omega',
+  Omega; Gamma |- M ::: A @ w ->
+  Omega *=* Omega' ->
+  Omega'; Gamma |- M ::: A @ w.
+Admitted.
+
+Lemma PermutGamma:
+forall Omega Gamma M A w Gamma',
+  Omega; Gamma |- M ::: A @ w ->
+  Gamma *=* Gamma' ->
+  Omega; Gamma' |- M ::: A @ w.
+Admitted.
+
+Lemma subst_t_types_preserv:
+forall Omega Gamma M A B w N x,
+  lc_w_L N -> lc_t_L N ->
+  Omega; (w, (x, B)) :: Gamma |- M ::: A @ w ->
+  Omega; nil |- N ::: B @ w ->
+  Omega; Gamma |- [ N // fte x ] M ::: A @ w.
+intros.
+remember ((w, (x, B)):: Gamma) as Gamma'.
+induction H1; inversion HeqGamma'; subst; simpl in *.
+(* hyp *)
+case_if.
+inversion H3; subst.
+rewrite Mem_cons_eq in HT; destruct HT.
+  inversion H4; subst; replace Gamma with (nil ++ Gamma) by auto;
+  apply WeakeningGamma with (Gamma:=nil) (Gamma':=Gamma); rew_app; auto.
+  (*apply ok_L_smaller in Ok; auto.*) skip.
+  (*apply ok_L_Mem_contradiction. *) skip.
+constructor.
+  (*apply ok_L_smaller in Ok; auto.*) skip.
+  rewrite Mem_cons_eq in HT; destruct HT;
+  [inversion H4; subst; elim H3 | ]; auto.
+(* lam *)
+apply t_lam_L with (L:=L).
+  (*apply ok_L_smaller in Ok; auto.*) skip.
+  intros; unfold open_t_L in *.
+Admitted.
+
+Lemma rename_w_types_preserv_in_old:
+forall Omega Gamma M A w0 w1,
+  Omega; Gamma |- M ::: A @ w1 ->
+  Omega; Gamma |- {{ fwo w0 // fwo w1 }} M ::: A @ w0.
+Admitted.
+
+Lemma rename_w_types_preserv_in_new:
+forall Omega Gamma M A w0 w1,
+  w1::Omega; Gamma |- M ::: A @ w0 ->
+  Omega; Gamma |- {{ fwo w0 // fwo w1 }} M ::: A @ w0.
+Admitted.
 
 Lemma Progress:
 forall Omega M A w
@@ -133,11 +288,100 @@ forall Omega M A w
   (H_lc': lc_t_L M)
   (HProgress: Omega; nil |- M ::: A@w),
   value_L M \/ exists N, (M, fwo w) |-> (N, fwo w).
-Admitted.
+induction M; intros; eauto using value_L; inversion HProgress; subst.
+(* hyp *)
+rewrite Mem_nil_eq in HT; contradiction.
+(* lam *)
+right; inversion H_lc; inversion H_lc'; subst;
+destruct (IHM1 (A0 ---> A) w H2 H7 HT1).
+  inversion H; subst; inversion HT1; subst.
+  inversion H2; inversion H7; subst;
+  eexists; constructor; eauto. apply lc_t_subst; auto.
+  destruct H; eexists; constructor; eauto.
+(* unbox *)
+right; inversion H_lc; inversion H_lc'; subst.
+destruct (IHM ([*]A) w H1 H4 HT).
+  inversion H; subst; inversion HT; subst.
+  inversion H1; inversion H4; subst; eexists; constructor; eauto.
+  apply lc_w_subst; auto.
+  destruct H; eexists; constructor; eauto.
+(* get *)
+right; inversion H_lc; inversion H_lc'; subst.
+destruct (IHM (<*>A0) w0 H1 H5 HT).
+  inversion H; subst; inversion HT; subst.
+    inversion H1; inversion H5; subst.
+    eexists; apply red_get_val_L; eauto.
+  destruct H; eexists; constructor; eauto.
+(* letd *)
+right; inversion H_lc; inversion H_lc'; subst.
+destruct (IHM1 (<*>A0) w H3 H8 HT1).
+  inversion H; subst; inversion HT1; subst.
+  inversion H3; inversion H8; subst;
+  eexists; constructor; eauto.
+  apply lc_t_subst; auto.
+  apply lc_w_subst; auto.
+  destruct H; eexists; constructor; eauto.
+  apply lc_t_subst; auto.
+  apply lc_w_subst; auto.
+(* here *)
+inversion H_lc; inversion H_lc'; subst.
+destruct (IHM A0 w H1 H4 HT).
+  left; constructor; auto.
+  right; destruct H; eexists; constructor; eauto.
+(* fetch *)
+right; inversion H_lc; inversion H_lc'; subst.
+destruct (IHM ([*]A0) w0 H1 H5 HT).
+  inversion H; subst; inversion HT; subst.
+    inversion H1; inversion H5; subst.
+    eexists; apply red_fetch_val_L; eauto.
+  destruct H; eexists; constructor; eauto.
+Qed.
 
 Lemma Preservation:
 forall Omega M N A w w'
   (HType: Omega; nil |- M ::: A@w)
   (HStep: (M, fwo w) |-> (N,fwo w')),
   Omega; nil |- N ::: A@w'.
-Admitted.
+intros; remember (@nil (prod var (prod var ty))) as Gamma;
+generalize dependent N; generalize dependent w';
+induction HType; intros; inversion HStep; subst; eauto using types_L.
+(* red_appl_lam *)
+inversion HType1; subst; unfold open_t_L in *.
+assert (exists x, x \notin L \u used_vars_term_L M0) as HF by apply Fresh.
+destruct HF as (v_f).
+replace ([N // bte 0] M0) with ([N // fte v_f] ([hyp_L (fte v_f) // bte 0] M0)).
+apply subst_t_types_preserv with (B:=A); auto.
+rewrite <- subst_t_neutral_free with (n:=0); auto.
+(* red_unbox_box *)
+inversion HType; subst; unfold open_w_L in *;
+assert (exists x, x \notin L \u used_worlds_term_L M0) as HF by apply Fresh;
+destruct HF as (w_f).
+replace ({{fwo w'//bwo 0}}M0) with ({{fwo w'//fwo w_f}}{{fwo w_f//bwo 0}}M0).
+apply rename_w_types_preserv_in_new.
+apply HT; auto.
+rewrite <- subst_w_neutral_free with (n:=0); auto.
+(* red_fetch_val *)
+apply rename_w_types_preserv_in_old; auto.
+(* red_get_here *)
+inversion HType; subst; constructor; auto;
+apply rename_w_types_preserv_in_old; auto.
+(* red_letd_here *)
+clear H.
+inversion HType; subst; unfold open_w_L in *; unfold open_t_L in *;
+assert (exists x, x \notin Lt \u used_vars_term_L {{fwo w' // bwo 0}}N)
+  as HF by apply Fresh;
+destruct HF as (v_f).
+assert (exists x, x \notin Lw \u used_worlds_term_L [hyp_L (fte v_f) // bte 0]N)
+  as HF by apply Fresh;
+destruct HF as (w_f).
+replace ([M0 // bte 0] ({{fwo w' // bwo 0}}N)) with
+  ([M0 // fte v_f] ([hyp_L (fte v_f) // bte 0] ({{fwo w'// bwo 0}} N)))
+  by (rewrite <- subst_t_neutral_free; auto);
+apply subst_t_types_preserv with (B:=A); auto.
+rewrite <- subst_order_irrelevant_bound; [ | constructor];
+replace ( {{fwo w' // bwo 0}}([hyp_L (fte v_f) // bte 0]N)) with
+  ({{fwo w' // fwo w_f}} ({{fwo w_f // bwo 0}} ([hyp_L (fte v_f) // bte 0] N)))
+  by (rewrite <- subst_w_neutral_free; auto);
+apply rename_w_types_preserv_in_new;
+rewrite subst_order_irrelevant_bound; auto; constructor.
+Qed.
