LLSubstitution.v
@@ -6,7 +6,7 @@ Global Reserved Notation " [ M // v ] N " (at level 5).
 (* Notation for world substitution *)
 Global Reserved Notation " {{ w1 // w2 }} N " (at level 5).
 
-Fixpoint subst_t (M0: te_L) (v0: vte) (N0: te_L) :=
+Fixpoint subst_t_L (M0: te_L) (v0: vte) (N0: te_L) :=
 match N0 with
 | hyp_L v =>
     if (eq_vte_dec v v0) then M0 else N0
@@ -27,9 +27,9 @@ match N0 with
 | letd_L M N =>
     letd_L ([M0//v0]M) ([M0//shift_vte v0]N)
 end
-where " [ M // v ] N " := (subst_t M v N) : labeled_is5_scope.
+where " [ M // v ] N " := (subst_t_L M v N) : labeled_is5_scope.
 
-Fixpoint subst_w (M0: te_L) (w1: vwo) (w2: vwo) :=
+Fixpoint subst_w_L (M0: te_L) (w1: vwo) (w2: vwo) :=
 match M0 with
 | hyp_L n => hyp_L n
 | lam_L A M => lam_L A ({{w1//w2}}M)
@@ -46,11 +46,50 @@ match M0 with
 | letd_L M N =>
     letd_L ({{w1//w2}} M) ({{shift_vwo w1 // shift_vwo w2}} N)
 end
-where " {{ w1 // w2 }} M " := (subst_w M w1 w2) : labeled_is5_scope.
+where " {{ w1 // w2 }} M " := (subst_w_L M w1 w2) : labeled_is5_scope.
 
-Definition open_t (M: te_L) (t: te_L) := subst_t t (bte 0) M.
+Definition open_t_L (M: te_L) (t: te_L) := subst_t_L t (bte 0) M.
 
-Definition open_w M w := subst_w M w (bwo 0).
+Definition open_w_L M w := subst_w_L M w (bwo 0).
 
-Notation " M '^t^' t " := (open_t M t) (at level 5) : labeled_is5_scope.
-Notation " M ^w^ w  " := (open_w M w) (at level 10) : labeled_is5_scope.
+Notation " M '^t^' t " := (open_t_L M t) (at level 5) : labeled_is5_scope.
+Notation " M '^w^' w  " := (open_w_L M w) (at level 10) : labeled_is5_scope.
+
+Open Scope labeled_is5_scope.
+
+Lemma subst_t_neutral_free:
+forall M N n w,
+  w \notin used_vars_term_L M ->
+  [N // bte n] M = [N // fte w] ([hyp_L (fte w) // bte n] M).
+Admitted.
+
+Lemma subst_w_neutral_free:
+forall M n w w_f,
+  w_f \notin used_worlds_term_L M ->
+  {{w // bwo n}} M = {{w // fwo w_f}} ({{ fwo w_f // bwo n}}  M).
+Admitted.
+
+Lemma subst_order_irrelevant_free:
+forall M w0 w1 x N,
+  w1 \notin used_worlds_term_L M ->
+  {{ w0 // fwo w1 }} ([ N // x ] M) = [ N // x ] ({{ w0 // fwo w1 }} M).
+Admitted.
+
+Lemma subst_order_irrelevant_bound:
+forall M w0 w1 x N,
+  lc_w_L N ->
+  {{ w0 // bwo w1 }} ([ N // x ] M) = [ N // x ] ({{ w0 // bwo w1 }} M).
+Admitted.
+
+Lemma lc_t_subst:
+forall M N k,
+  lc_t_n_L (S k) M ->
+  lc_t_n_L 0 N ->
+  lc_t_n_L k [N // bte k] M.
+Admitted.
+
+Lemma lc_w_subst:
+forall M w k,
+  lc_w_n_L (S k) M ->
+  lc_w_n_L k {{w // bwo k}} M.
+Admitted.
