LLOkLib.v
@@ -1,0 +1,52 @@
+Require Import LLSyntax.
+Require Import PermutLib.
+
+Open Scope permut_scope.
+
+Fixpoint ok_Gamma (G: Context_L) (Used: list var) : Prop :=
+match G with
+| nil => True
+| (w, (v, A)) :: G' => ~ Mem v Used /\ ok_Gamma G' (v::Used)
+end.
+
+Fixpoint ok_Omega (L: list var) : Prop :=
+match L with
+| nil => True
+| l :: L' => ~ Mem l L' /\ ok_Omega L'
+end.
+
+Lemma ok_Gamma_permut:
+forall G1 G2 U,
+  G1 *=* G2 -> ok_Gamma G1 U -> ok_Gamma G2 U.
+Admitted.
+
+Lemma ok_Omega_permut:
+forall O1 O2,
+  O1 *=* O2 -> ok_Omega O1 -> ok_Omega O2.
+Admitted.
+
+Definition ok_L Omega Gamma := ok_Omega Omega /\ ok_Gamma Gamma nil.
+
+Lemma ok_L_permut:
+forall O O' G G', O *=* O' -> G *=* G' -> ok_L O G -> ok_L O' G'.
+intros; destruct H1; split;
+[eapply ok_Omega_permut | eapply ok_Gamma_permut]; eauto.
+Qed.
+
+Lemma ok_L_extend_fresh:
+forall O G x w A,
+  ok_L O G ->
+  x \notin used_vars_context_L G ->
+  ok_L O ((w, (x, A))::G).
+Admitted.
+
+Lemma ok_L_smaller:
+forall O G x w A,
+  ok O ((w, (x, A))::G) -> ok O G.
+Admitted.
+
+Lemma ok_L_Mem_contradiction:
+  Mem (w, (x, A)) Gamma ->
+  ok_L Omega ((w, (x, B)) :: Gamma) ->
+  False.
+Admitted.
